@@ -6,8 +6,13 @@ import Xv6.ProofAcquiresleep
 
 namespace Xv6
 
-theorem Acquiresleep (AC : ACQUIRE) (RE : RELEASE) (MP : MYPROC) (SP : SLEEP_PREPARE)
-    (SL : SLEEP) : ACQUIRESLEEP := acquiresleep_proof AC RE MP SP SL
+/-- The store-order form (the primitive one): the acquire edge's receipt,
+cashed into `MachCSL.ctxFloor curCtx tl`. -/
+theorem AcquiresleepLlb (ACL : ACQUIRE_LLB) (RE : RELEASE) (MP : MYPROC) (SP : SLEEP_PREPARE)
+    (SL : SLEEP) : ACQUIRESLEEP_LLB := acquiresleep_llb_proof ACL RE MP SP SL
+
+theorem Acquiresleep (ACL : ACQUIRE_LLB) (RE : RELEASE) (MP : MYPROC) (SP : SLEEP_PREPARE)
+    (SL : SLEEP) : ACQUIRESLEEP := (AcquiresleepLlb ACL RE MP SP SL).toACQUIRESLEEP
 
 theorem AcquiresleepNb (AC : ACQUIRE) (RE : RELEASE) (MP : MYPROC) : ACQUIRESLEEP_NB :=
   acquiresleep_nb_proof AC RE MP
